src/cddl/spec/CDDL.Spec.MapGroup.Base.fst
@@ -2017,7 +2017,7 @@ let t_map_eq
   g x
 = ()
 
-#push-options "--z3rlimit 16"
+#push-options "--z3rlimit 32"
 
 let t_map_ext g1 g2 =
   assert (FE.feq (t_map' g1) (t_map' g2))
